theories/Util/Wf_Uint63/Proofs.v
@@ -27,210 +27,116 @@ Module Reduction.
     break_innermost_match; eauto.
   Qed.
 
-  Lemma map_reduce_no_init_spec {A reduce start0 stop step0 f} (P : int -> A -> Prop)
+  Lemma map_reduce_no_init_spec_count {A reduce start stop step0 f} (P : nat -> int -> _ -> Prop)
     (step : int := if (step0 =? 0) then 1 else step0)
-    (start : int := start0 + step)
-    (Hinit : P start (f start0))
-    (Hstep : forall i v, P i v -> ((i + step) <? stop) = true -> P (i + step) (reduce v (f i)))
-    : P (start + step * (if start <? stop then (stop - start - 1) // step else 0))
-        (@map_reduce_no_init A reduce start0 stop step0 f).
+    (Hinit : P 1 (start + step) (f start))
+    (Hstep : forall n i v, P (S n) i v -> (start + step <=? i) = true -> (i <? stop) = true -> i = start + step + step * Uint63.of_Z n -> P (S (S n)) (i + step) (reduce v (f i)))
+    : P (S (if start + step <? stop then (1 + Z.to_nat ((stop - (start + step) - 1) // step : int)) else 0))
+        (start + step + step * (if start + step <? stop then 1 + (stop - (start + step) - 1) // step else 0))
+        (@map_reduce_no_init A reduce start stop step0 f).
   Proof.
-    cbv [map_reduce_no_init start].
-    eapply for_loop_lt_invariant_gen
-      with (P:=fun i v
-               => P i v
-                  /\ ((i - start) mod step) = 0
-                  /\ (start <=? i) = true
-                  /\ ((start <? stop) = true -> i = start \/ ((i - step) <? stop) = true)
-                  /\ ((start <? stop) = false -> i = start)).
-    all: cbv [run_body Monad.bind LoopBody_Monad bind LoopNotation.get LoopNotation.set LoopNotation.update Classes.modulo Classes.sub Classes.add Classes.ltb int_has_modulo int_has_sub int_has_ltb int_has_leb Classes.leb int_has_add Classes.eqb int_has_eqb Classes.zero Classes.one int_has_zero int_has_one int_has_int_div Classes.int_div Classes.mul int_has_mul] in *.
-    { repeat apply conj; try assumption; subst step start; break_innermost_match.
-      all: lazymatch goal with
-           | [ |- ((?x mod ?y) = 0)%uint63 ]
-             => first [ replace x with y by lia | replace x with 0%uint63 by lia ];
-                assert (y / y = 1 /\ 0 / y = 0)%uint63; nia
-           | _ => try lia
-           end. }
-    3: { subst step start; break_innermost_match; intros; destruct_head'_and.
-         all: repeat match goal with H : _ |- _ => specialize (H eq_refl) end.
-         all: destruct_head'_or; subst.
-         all: try match goal with
-                | [ H : ?P ?x ?v |- ?P ?y ?v ] => replace y with x by lia
-                | [ H1 : (?x - 1 <? ?y)%uint63 = true, H2 : (?x <? ?y)%uint63 = false |- _ ] => assert (x = y) by (clear -H1 H2; lia); clear H1 H2; subst
-                end.
-         all: try assumption.
-         (*
-         3: {
-         assert (start = (start + step0) - step0)%uint63 by lia.
-         generalize dependent (start + step0)%uint63; intro start'; intros; subst.
-         assert (i = start + (i - start))%uint63 by lia.
-         generalize dependent (i - start)%uint63; intro i'; intros; subst.
-         assert (stop = start + (stop - start))%uint63 by lia.
-         generalize dependent (stop - start)%uint63; intro len; intros; subst.
-         match goal with
-         | [ H : (?x mod ?y = 0)%uint63 |- _ ]
-           => let H' := fresh in
-              is_var x;
-              assert (y <> 0%uint63) by lia;
-              assert (x = y * (x / y))%uint63 by (clear -H H'; nia);
-              clear H;
-              generalize dependent (x / y)%uint63;
-              let x' := fresh in
-              rename x into x';
-              intro x; intros; subst
+    cbv [map_reduce_no_init for_loop_lt Fix Classes.eqb int_has_eqb Classes.one Classes.zero int_has_one int_has_zero Classes.leb Classes.ltb int_has_leb int_has_leb int_has_ltb nat_has_zero nat_has_one Classes.add int_has_add] in *.
+    fold step.
+    set (f' := fun (i : int) continue state => _) at 1.
+    set (wf := Acc_intro_generator _ _ _); clearbody wf.
+    set (start' := (start + step)%uint63) in *.
+    generalize dependent (f start); intro init; intros.
+    clearbody start'; clear start; rename start' into start.
+    set (start0 := start) in Hstep.
+    assert (Hstart : (start0 <=? start) = true) by (cbv; lia).
+    set (n0 := O) in Hinit.
+    assert (Hn : start = start0 + step * Uint63.of_Z n0) by (cbv; lia).
+    change (P ?x) with (P (n0 + x)%nat).
+    clearbody start0 n0.
+    revert start wf init Hstart n0 Hn Hinit.
+    fix IH 2.
+    intros ? [wf]; intros; cbn [Fix_F]; cbv [Acc_inv].
+    unfold f' at 1.
+    set (wf' := wf _); specialize (fun pf y b => IH _ (wf' y) b pf); clearbody wf'; clear wf.
+    cbv [Monad.bind run_body LoopNotation.get LoopBody_Monad bind LoopNotation.set LoopNotation.update].
+    cbv [Classes.sub Classes.mul Classes.zero Classes.add Classes.ltb Classes.leb Classes.one Classes.int_div int_has_int_div int_has_sub int_has_ltb int_has_add int_has_mul int_has_leb] in *.
+    break_match; break_innermost_match_hyps; auto.
+    all: try (specialize (IH ltac:(lia))).
+    all: lazymatch goal with
+         | [ H : (?start <? ?stop)%uint63 = true, H' : (?step <? ?stop - ?start)%uint63 = false |- context[((?stop - ?start - 1) / ?step)%uint63] ]
+           => let H'' := fresh in
+              let H''' := fresh in
+              assert (H'' : (stop - start - 1 <? step)%uint63 = true) by lia;
+              assert (H''' : (0 <? step)%uint63 = true) by lia;
+              replace ((stop - start - 1) / step)%uint63 with 0%uint63 by (clear -H'' H'''; nia)
+         | _ => idtac
          end.
-         assert (len = (len - 1) + 1)%uint63 by lia.
-         generalize dependent (len - 1)%uint63; intro len'; intros; subst.
-         assert ((step0 <=? step0 * i')%uint63 = true) by lia.
-         assert (len' = step0 * (len' / step0) + (len' mod step0))%uint63 by (clear; nia).
-         generalize dependent (len' / step0)%uint63; intro len; intros; subst.
-         assert ((0 <=? len' mod step0) = true)%uint63 by (clear; nia).
-         let H := lazymatch goal with H : step0 <> 0%uint63 |- _ => H end in
-         assert ((len' mod step0 <? step0) = true)%uint63 by (clear -H; nia).
-         generalize dependent (len' mod step0)%uint63; intro lenmod; intros; subst.
-         assert ((step0 * i' - step0 <? step0 * len + lenmod + 1) = true)%uint63 by lia.
-         match goal with
-                | [ H : ?P ?x ?v |- ?P ?y ?v ] => replace y with x by nia
-                end.
-         assert (step0
-         nia.
-         zify.
-         assert (
-         assert (
-         match goal with
-                | [ H : ?P ?x ?v |- ?P ?y ?v ] => replace y with x by nia
-                end.
-         assert (
-         nia.
+    all: lazymatch goal with
+         | [ |- context[(?x * (1 + 0))%uint63] ]
+           => replace (x * (1 + 0))%uint63 with x by lia
+         | _ => idtac
+         end.
+    all: rewrite ?Nat.add_0_r.
+    all: try match goal with
+           | [ H : ?P _ ?x ?v |- ?P _ ?y ?v ] => replace y with x by lia
+           end.
+    all: try assumption.
+    all: try match goal with |- ?P (?n + ?x)%nat _ _ => change x with 1%nat end.
+    all: rewrite ?Nat.add_succ_r, ?Nat.add_0_r.
+    all: auto.
+    all: try (exfalso; lia).
+    all: [ > ].
+    do 3 (let x := open_constr:(_) in specialize (IH x)).
+    lazymatch goal with
+    | [ |- ?P ?n ?y ?v ]
+      => lazymatch type of IH with
+         | _ -> _ -> P ?n' ?x ?v'
+           => unify v v';
+              replace y with x;
+              [ replace n with n'
+              | ]
+         end
+    end.
+    { specialize (fun pf => IH pf ltac:(eauto)).
+      specialize (IH ltac:(lia)).
+      auto. }
+    all: match goal with
+         | [ |- context[((?stop - (?start + ?step) - 1) / ?step)%uint63] ]
+           => replace ((stop - (start + step) - 1))%uint63 with (((stop - start - 1) - step))%uint63 by lia
+         end.
+    all: match goal with
+         | [ |- context[((?x - ?z) / ?z)%uint63] ]
+           => let H := fresh in
+              let H' := fresh in
+              assert (H : z <> 0%uint63) by (subst z; clear; break_innermost_match; lia);
+              assert (H' : (z <=? x)%uint63 = true) by lia;
+              replace ((x - z) / z)%uint63 with (x / z - 1)%uint63;
+              [
+              | revert H H'; generalize x z; clear;
+                intros;
+                zify;
+                let wBv := (eval cbv in wB) in
+                repeat match goal with
+                  | [ H : context[(wBv * ?q)%Z] |- _ ]
+                    => lazymatch goal with
+                       | [ H' : (q = 0 \/ q = 1)%Z |- _ ] => fail
+                       | [ H' : (q = 0 \/ q = -1)%Z |- _ ] => fail
+                       | _ => first [ assert (q = 0 \/ q = 1)%Z by nia
+                                    | assert (q = 0 \/ q = -1)%Z by nia ]
+                       end
+                  end ]
+         end;
+      [ | nia ].
+    2: lia.
+    { assert ((0 <? (stop - start - 1) / step)%uint63 = true) by lia.
+      generalize dependent (((stop - start - 1) / step)%uint63); intros.
+      lia. }
+  Qed.
 
-         Ltac zify_convert_to_euclidean_division_equations_flag ::= constr:(false).
-         zify.
-         rewrite Z.div_1_r.
-         rewrite Z.mul_1_l.
-         rewrite !Z.mod_mod by lia.
-
-         Ltac zify_convert_to_euclidean_division_equations_flag ::= constr:(true).
-         zify.
-         nia.
-         lia.
-
-         Z.to_euclidean_division_equations_
-         zify.
-
-         zify.
-         2: lia.
-         zify.
-      lia.
-      lia.
-      lia.
-      lia.
-      { clear.
-        subst step; break_innermost_match.
-        nia.
-        transitivity (step0 mod step0)%uint63; [ f_equal; lia | ].
-        assert (step0 / step0 = 1)%uint63; nia. }
-      subst step.
-
-    }
-
-      {
-      zify.
-      clear H3 H2.
-      clear H1.
-      specialize (H0 ltac:(lia)).
-      specialize (H ltac:(lia)).
-      generalize dependent (to_Z step0); clear step0; intros.
-
-      nia.
-
-      nia.
-      zify; lia.
-      zify.
-      nia.
-      zify. nia.
-      zify; Z.to_euclidean_division_equations; try nia.
-      break_innermost_match_hyps; subst; zify; try lia.
-      generalize dependent (to_Z step0); clear step0; intro step0; intros.
-      generalize dependent (to_Z step); clear step; intro step; intros.
-      generalize dependent (to_Z start); clear start; intro start; intros.
-      subst.
-      repeat match goal with H : _ |- _ => specialize (H ltac:(lia)) end.
-      assert (step0 <> 0)%Z by lia.
-      clear Heqb H3 H2.
-      clear H1.
-      clear H7 H6.
-      clear H11 H12.
-      subst.
-      clear H8.
-      clear H13.
-      assert (r1 = start + step0 - 9223372036854775808 * q1)%Z by lia.
-      clear H9.
-      subst.
-      assert ((step0 * (1 - q) - 9223372036854775808 * (q1 + q0) - ( r)%Z) = 0%Z)%Z by nia.
-      clear H4.
-      assert (0 <= q1 <= 1)%Z by nia.
-      assert (0 <= q0 + q1 <= 1)%Z by nia.
-      assert (-1 <= q0 <= 0)%Z by nia.
-      assert (0 <= q <= 1)%Z by nia.
-      assert (0 = q \/ 1 = q)%Z by lia.
-      destruct_head'_or; subst; lia.
-      assert (q0 + q1 = 0%Z) by nia.
-      assert (q0 = 0) by nia.
-      assert (q1 = 0) by nia.
-      nia.
-      subst.
-      clear H3 H2 H1.
-      clear Heqb cstr.
-      lia.
-      assert (r
-
-      zify.
-      zify.
-
-      Set Printing All.
-      zify.
-      assert (step0 = 0%Z).
-      Set Printing All.
-      zify.
-      Print Ltac Zify.zify.
-
-      { clear H13.
-        repeat match goal with H : _ |- _ => clear H; assert_succeeds (zify; [ | ]) end.
-        exfalso.
-        repeat match goal with H : _ |- _ => clear H; assert_succeeds (zify; [ | ]) end.
-        generalize dependent (@eqb int int_has_eqb); intro f; intros.
-        rename step0 into x.
-        assert
-        revert x f cstr4.
-  zify.
-  lia.
-
-
-        zify.
-        assert (step0 = 0%uint63).
-        Set Printing All.
-        zify.
-        zify.
-        zify.
-        zify.
-        zify.
-        Zify.zify_op.
-        Zify.zify_op.
-      Print Ltac zify.
-      zify.
-      zify.
-      zify.
-      zify.
-      zify.
-      zify.
-      zify.
-    Set Printing All.
-
-    eassumption.
-    Print for_loop_lt.
-    revert dependent start.
-          *)
-  Abort.
+  Lemma map_reduce_no_init_spec {A reduce start stop step0 f} (P : int -> _ -> Prop)
+    (step : int := if (step0 =? 0) then 1 else step0)
+    (Hinit : P (start + step) (f start))
+    (Hstep : forall i v, P i v -> (start + step <=? i) = true -> (i <? stop) = true -> P (i + step) (reduce v (f i)))
+    : P (start + step + step * (if start + step <? stop then 1 + (stop - (start + step) - 1) // step else 0))
+        (@map_reduce_no_init A reduce start stop step0 f).
+  Proof.
+    eapply map_reduce_no_init_spec_count with (P := fun _ => P); eauto.
+  Qed.
 
   Lemma map_reduce_spec_count {A B reduce init start stop step0 f} (P : nat -> int -> _ -> Prop)
     (step : int := if (step0 =? 0) then 1 else step0)
@@ -340,69 +246,70 @@ Module Reduction.
     eapply map_reduce_spec_count with (P := fun _ => P); eauto.
   Qed.
 
-  Lemma argmax_gen_spec {A} {ltbA : has_ltb A} {start stop step f i v}
-    (Hstep : step <> 0)
-    : map_reduce_no_init (@argmax_ int A ltbA) start stop step (fun i : int => (i, f i)) = (i, v)
-      <-> (v = f i /\ forall j, (f j <? f i) = true).
-  Proof.
-    assert (to_Z step <> 0) by now intro; apply Hstep; apply to_Z_inj.
-    cbv [map_reduce_no_init].
-    set (v' := (start, f start)).
-    assert (Hv'' : f (fst v') = snd v' /\ forall j, (j <? ((start + step) - start) // step) = true -> let fv' := f (start + j * step) in fv' = snd v' \/ (fv' <? snd v') = true).
-    { split; [ reflexivity | intros j H'; left; subst v'; cbn; apply f_equal, to_Z_inj ].
-      cbv in H'; revert H'.
-      rewrite !ltb_spec, !div_spec, !sub_spec, !add_spec, !mul_spec.
-      repeat match goal with |- context[to_Z ?x] => unique pose proof (to_Z_bounded x) end.
-      rewrite Zminus_mod_idemp_l, Z.add_simpl_l, Z.mod_small by lia.
-      rewrite Z.div_same by assumption.
-      intro; assert (Hz : to_Z j = to_Z 0) by (transitivity 0%Z; try reflexivity; lia).
-      apply to_Z_inj in Hz; subst.
-      rewrite to_Z_0, Z.mul_0_l, Z.mod_0_l, Z.add_0_r, Z.mod_small by lia.
-      reflexivity. }
-    clearbody v'.
-(*
-      rewrite
-      left.
-      f_equal.
-      2: {
-      rewrite Z.mod_small
-      Search (?x + ?y - ?x)%Z.
-      Search (((_ mod _) - _) mod _)%Z.
-      push_Zmod.
-      intros.
-
-      intros
-    set (fv := f start).
-    assert (fv
-    apply for_loop_lt_invariant_gen with (P := fun i' v => forall j,
-    cbv [argmax].
-    cut
-  Lemma argmax_gen_spec {A} {ltbA : has_ltb A} {start stop step f i v}
-    : map_reduce_no_init (@argmax_ int A ltbA) start stop step (fun i : int => (i, f i)) = (i, v)
-      <-> (v = f i /\ forall j, (f j <? f i) = true).
-  Proof.
-    cbv [map_reduce_no_init].
-    apply for_loop_lt_invariant_gen.
-    cbv [argmax].
-    cut
-  Lemma argmax_spec {A} {ltbA : has_ltb A} {start stop step f v}
-    : @argmax A ltbA start stop step f = v
-      <-> forall j, (f j <? f v) = true.
-  Proof.
-    cbv [argmax].
-    cut
-    cbv [map_reduce_no_init].
-
-  Lemma argmax_spec {A} {ltbA : has_ltb A} {start stop step f v}
-    : @argmax A ltbA start stop step f = v
-      <->
-    (start : int) (stop : int) (step : int) (f : int -> A) : int
-    := fst (map_reduce_no_init argmax_ start stop step (fun i => (i, f i))).
- *)
-  Abort.
-
   Definition in_bounds (start stop step i : int) : bool
     := ((start <=? i) && ((i =? start) || (i <? stop)) && (((i - start) mod step) =? 0)).
+
+  Lemma argmax_gen_spec {A} {ltbA : has_ltb A} {start stop step0 f i v}
+    (step : int := if (step0 =? 0) then 1 else step0)
+    : map_reduce_no_init (@argmax_ int A ltbA) start stop step0 (fun i : int => (i, f i)) = (i, v)
+      <-> (v = f i
+           /\ (exists n : nat,
+                  (n <= Nat.pred (S (if start + step <? stop then (1 + Z.to_nat ((stop - (start + step) - 1) // step : int)) else 0)))
+                  /\ i = start + step * Uint63.of_Z n)
+           /\ forall j,
+              (exists n : nat,
+                  (n <= Nat.pred (S (if start + step <? stop then (1 + Z.to_nat ((stop - (start + step) - 1) // step : int)) else 0)))
+                  /\ j = start + step * Uint63.of_Z n)
+              -> (((f j <? f i) = true)
+                  \/ (f j = f i /\ (i <=? j) = true))).
+  Proof.
+    revert v i.
+    apply map_reduce_no_init_spec_count with (P:=fun n _ v => forall v' i', v = _ <-> _).
+    all: fold step.
+    all: intros; cbv [argmax_]; cbn [fst snd]; break_innermost_match; split; intros.
+    all: cbv [Classes.one Classes.zero Classes.add Classes.mul nat_has_one int_has_one int_has_add int_has_mul int_has_zero Nat.lt] in *.
+    all: repeat first [ progress subst
+                      | progress change (of_Z 0%nat) with 0%uint63 in *
+                      | progress intros
+                      | reflexivity
+                      | progress cbn [fst snd Nat.pred] in *
+                      | match goal with
+                        | [ H : (_, _) = (_, _) |- _ ] => inversion H; clear H
+                        | [ H : _ /\ _ |- _ ] => destruct H
+                        | [ H : ex _ |- _ ] => destruct H
+                        | [ H : ?x <= 0%nat |- _ ] => assert (x = 0%nat) by lia; subst; clear H
+                        | [ |- context[(?x * 0)%uint63] ] => replace (x * 0)%uint63 with 0%uint63 by lia
+                        | [ |- context[(?x + 0)%uint63] ] => replace (x + 0)%uint63 with x by lia
+                        | [ |- ?x = ?x /\ _ ] => split
+                        | [ |- 0%nat < 1%nat ] => lia
+                        | [ |- _ /\ ?x = ?x ] => split
+                        | [ |- (exists n, n <= 0%nat /\ _) /\ _ ] => split; [ exists 0%nat | ]
+                        | [ |- (?x <? ?x) = true \/ _ ] => right
+                        | [ |- (?x <=? ?x) = true ] => generalize x; cbv; clear; intros; lia
+                        | [ H : _ * _ |- _ ] => destruct H
+                        | [ H : forall v' i', (?i, ?v) = (i', v') <-> _ |- _ ]
+                          => pose proof (proj1 (H _ _) eq_refl);
+                             pose proof (fun v' i' => proj2 (H v' i'));
+                             clear H
+                        | [ H : forall v' i', v' = _ /\ _ -> _ |- _ ] => specialize (fun i' pf => H _ i' (conj eq_refl pf))
+                        | [ |- _ /\ _ ] => split
+                        | [ |- context[(?start + ?step + ?step * of_Z (Z.of_N (N.of_nat ?n')))%uint63] ]
+                          => replace (start + step + step * of_Z (Z.of_N (N.of_nat n')))%uint63
+                            with (start + step * of_Z (Z.of_N (N.of_nat (S n'))))%uint63 in *
+                            by lia
+                        | [ |- exists n, _ /\ (?start + ?step * of_Z (Z.of_N (N.of_nat ?n')) = ?start + ?step * of_Z (Z.of_N (N.of_nat n)))%uint63 ]
+                          => exists n'
+                        | [ H : forall j, ex _ -> (?f j <? ?f ?x) = true \/ _, H' : (?f ?x <? ?f ?y) = true |- (?f ?z <? ?f ?y) = true \/ _ ]
+                          => specialize (fun pf => H z (ex_intro _ _ (conj pf eq_refl)))
+                        | [ H : ?x <= ?y -> _, H' : ?x <= S ?y |- _ ]
+                          => is_var x; destruct (Nat.eq_decidable x (S y)); subst;
+                             [ clear H H'
+                             | assert (x <= y) by lia;
+                               clear H';
+                               specialize (H ltac:(assumption)) ]
+                        end
+                      | lia ].
+  Admitted.
 
   Lemma argmax_spec {A} {ltbA : has_ltb A} {start stop step f v}
     : @argmax A ltbA start stop step f = v
@@ -504,7 +411,8 @@ Module Reduction.
       {zeroA_mul_l : LeftZero R mul 0}
       {zeroA_mul_r : RightZero R mul 0}
       {mulA_addA_distr_l : LeftDistributive R mul add}
-      {mulA_addA_distr_r : RightDistributive R mul add}.
+      {mulA_addA_distr_r : RightDistributive R mul add}
+      {coerN : has_coer N A}.
 
     Lemma sum_const [start stop step] (f : A)
       : sum start stop step (fun x => f)
@@ -514,6 +422,22 @@ Module Reduction.
              else 0) (fun v : A => v + f) 0.
     Proof using Type.
       cbv [sum]. rewrite map_reduce_const; reflexivity.
+    Qed.
+
+    Lemma sum_const_mul
+      (H0l : forall x : A, R 0 (coer (0:N) * x))
+      (Hsucc : forall (x : A) (n : N), R (coer n * x + x) (coer (N.succ n) * x))
+      [start stop step] (f : A)
+      : R (sum start stop step (fun x => f))
+          (coer
+             (if start <? stop return N
+              then 1 + (((stop - start - 1) // (if step =? 0 then 1 else step) : int) : N)
+              else 0) * f).
+    Proof using R_refl R_trans addA_Proper.
+      rewrite sum_const.
+      set (n := if start <? stop then _ else _); clearbody n.
+      induction n as [|n IH] using N.peano_ind; [ now cbn; apply H0l | ].
+      rewrite N.iter_succ, IH; apply Hsucc.
     Qed.
 
     Lemma sum_const0 start stop step
@@ -535,6 +459,22 @@ Module Reduction.
       f_equal.
       replace ((stop - start - 1) / 1)%uint63 with (stop - start - 1)%uint63 by nia.
       lia.
+    Qed.
+
+    Lemma sum_const_mul_step1
+      (H0l : forall x : A, R 0 (coer (0:N) * x))
+      (Hsucc : forall (x : A) (n : N), R (coer n * x + x) (coer (N.succ n) * x))
+      [start stop] (f : A)
+      : R (sum start stop 1 (fun x => f))
+          (coer
+             (if start <? stop return N
+              then N.succ (stop - start - 1)%uint63
+              else 0) * f).
+    Proof using R_refl R_trans addA_Proper.
+      rewrite sum_const_step1.
+      set (n := if start <? stop then _ else _); clearbody n.
+      induction n as [|n IH] using N.peano_ind; [ now cbn; apply H0l | ].
+      rewrite N.iter_succ, IH; apply Hsucc.
     Qed.
 
     Lemma sum_distr [start stop step] (f g : int -> A)
